theories/VLSM/Core/VLSMProjections.v
@@ -1,5 +1,6 @@
 From Cdcl Require Import Itauto. Local Tactic Notation "itauto" := itauto auto.
 From stdpp Require Import prelude.
+From Coq Require Import FunctionalExtensionality.
 From VLSM.Lib Require Import Preamble ListExtras StreamExtras StreamFilters.
 From VLSM.Core Require Import VLSM.
 From VLSM.Core.VLSMProjections Require Export VLSMPartialProjection VLSMProjection.
@@ -24,3 +25,262 @@ Proof.
 Qed.
 
 End same_VLSM_full_projection.
+
+Section transitivity_props.
+
+Lemma pre_VLSM_projection_trace_project_trans
+  {message}
+  (TX TY TZ : VLSMType message)
+  (project_labelXY : @label _ TX -> option (@label _ TY))
+  (project_stateXY : @state _ TX -> @state _ TY)
+  (project_labelYZ : @label _ TY -> option (@label _ TZ))
+  (project_stateYZ : @state _ TY -> @state _ TZ)
+  : forall trX,
+    pre_VLSM_projection_trace_project TX TZ
+      (mbind project_labelYZ ∘ project_labelXY)
+      (project_stateYZ ∘ project_stateXY)
+      trX
+      =
+    pre_VLSM_projection_trace_project TY TZ project_labelYZ project_stateYZ
+      (pre_VLSM_projection_trace_project TX TY project_labelXY project_stateXY
+        trX).
+Proof.
+  induction trX; [done |]; destruct a; cbn;
+    unfold pre_VLSM_projection_transition_item_project; cbn;
+    unfold mbind, option_bind; cbn.
+  destruct (project_labelXY l) as [lY |]; [| done]; cbn;
+    unfold pre_VLSM_projection_transition_item_project; cbn.
+  destruct (project_labelYZ lY) as [lZ |]; [| done]; cbn.
+  by f_equal.
+Qed.
+
+Lemma VLSM_projection_trans
+  {message}
+  (X Y Z : VLSM message)
+  (project_labelXY : vlabel X -> option (vlabel Y))
+  (project_stateXY : vstate X -> vstate Y)
+  (ProjXY : VLSM_projection X Y project_labelXY project_stateXY)
+  (project_labelYZ : vlabel Y -> option (vlabel Z))
+  (project_stateYZ : vstate Y -> vstate Z)
+  (ProjYZ : VLSM_projection Y Z project_labelYZ project_stateYZ)
+  : VLSM_projection X Z
+    (mbind project_labelYZ ∘ project_labelXY)
+    (project_stateYZ ∘ project_stateXY).
+Proof.
+  constructor; [split |]; intros sX trX HtrX; cbn;
+    setoid_rewrite pre_VLSM_projection_trace_project_trans.
+  - rewrite <- !final_state_project; [done | apply ProjXY | done | apply ProjYZ |].
+    by eapply (VLSM_projection_finite_valid_trace_from ProjXY).
+  - by eapply (VLSM_projection_finite_valid_trace ProjYZ),
+      (VLSM_projection_finite_valid_trace ProjXY).
+Qed.
+
+Lemma VLSM_projection_embedding_trans
+  {message}
+  (X Y Z : VLSM message)
+  (project_labelXY : vlabel X -> option (vlabel Y))
+  (project_stateXY : vstate X -> vstate Y)
+  (ProjXY : VLSM_projection X Y project_labelXY project_stateXY)
+  (project_labelYZ : vlabel Y -> vlabel Z)
+  (project_stateYZ : vstate Y -> vstate Z)
+  (ProjYZ : VLSM_full_projection Y Z project_labelYZ project_stateYZ)
+  : VLSM_projection X Z
+    (fmap project_labelYZ ∘ project_labelXY)
+    (project_stateYZ ∘ project_stateXY).
+Proof.
+  apply VLSM_full_projection_is_projection in ProjYZ.
+  replace (fmap project_labelYZ ∘ project_labelXY)
+    with (mbind (λ l : vlabel Y, Some (project_labelYZ l)) ∘ project_labelXY).
+  - by apply VLSM_projection_trans.
+  - by extensionality x.
+Qed.
+
+Lemma VLSM_embedding_projection_trans
+  {message}
+  (X Y Z : VLSM message)
+  (project_labelXY : vlabel X -> vlabel Y)
+  (project_stateXY : vstate X -> vstate Y)
+  (ProjXY : VLSM_full_projection X Y project_labelXY project_stateXY)
+  (project_labelYZ : vlabel Y -> option (vlabel Z))
+  (project_stateYZ : vstate Y -> vstate Z)
+  (ProjYZ : VLSM_projection Y Z project_labelYZ project_stateYZ)
+  : VLSM_projection X Z
+    (project_labelYZ ∘ project_labelXY)
+    (project_stateYZ ∘ project_stateXY).
+Proof.
+  apply VLSM_full_projection_is_projection in ProjXY.
+  replace (project_labelYZ ∘ project_labelXY)
+    with (mbind project_labelYZ ∘ (λ l : vlabel X, Some (project_labelXY l))).
+  - by apply VLSM_projection_trans.
+  - by extensionality x.
+Qed.
+
+Lemma pre_VLSM_full_projection_finite_trace_project_trans
+  {message}
+  (TX TY TZ : VLSMType message)
+  (project_labelXY : @label _ TX -> @label _ TY)
+  (project_stateXY : @state _ TX -> @state _ TY)
+  (project_labelYZ : @label _ TY -> @label _ TZ)
+  (project_stateYZ : @state _ TY -> @state _ TZ)
+  : forall trX,
+    pre_VLSM_full_projection_finite_trace_project TX TZ
+      (project_labelYZ ∘ project_labelXY)
+      (project_stateYZ ∘ project_stateXY)
+      trX
+      =
+    pre_VLSM_full_projection_finite_trace_project  TY TZ project_labelYZ project_stateYZ
+      (pre_VLSM_full_projection_finite_trace_project  TX TY project_labelXY project_stateXY
+        trX).
+Proof. by induction trX; [| destruct a; cbn; f_equal]. Qed.
+
+Lemma VLSM_embedding_trans
+  {message}
+  (X Y Z : VLSM message)
+  (project_labelXY : vlabel X -> vlabel Y)
+  (project_stateXY : vstate X -> vstate Y)
+  (ProjXY : VLSM_full_projection X Y project_labelXY project_stateXY)
+  (project_labelYZ : vlabel Y -> vlabel Z)
+  (project_stateYZ : vstate Y -> vstate Z)
+  (ProjYZ : VLSM_full_projection Y Z project_labelYZ project_stateYZ)
+  : VLSM_full_projection X Z
+    (project_labelYZ ∘ project_labelXY)
+    (project_stateYZ ∘ project_stateXY).
+Proof.
+  constructor; intros sX trX HtrX.
+  setoid_rewrite pre_VLSM_full_projection_finite_trace_project_trans.
+  by eapply (VLSM_full_projection_finite_valid_trace ProjYZ),
+    (VLSM_full_projection_finite_valid_trace ProjXY).
+Qed.
+
+Lemma VLSM_projection_incl_trans
+  {message}
+  (X : VLSM message)
+  {T : VLSMType message}
+  {MY MZ : VLSMMachine T}
+  (Y := mk_vlsm MY)
+  (Z := mk_vlsm MZ)
+  (project_labelXY : vlabel X -> option (vlabel Y))
+  (project_stateXY : vstate X -> vstate Y)
+  (ProjXY : VLSM_projection X Y project_labelXY project_stateXY)
+  (ProjYZ : VLSM_incl Y Z)
+  : VLSM_projection X Z project_labelXY project_stateXY.
+Proof.
+  replace project_labelXY with (fmap id ∘ project_labelXY)
+    by (extensionality lX; cbv; destruct (project_labelXY lX); done).
+  change project_stateXY with (id ∘ project_stateXY).
+  by apply (VLSM_projection_embedding_trans X Y Z); [| apply VLSM_incl_is_full_projection].
+Qed.
+
+Lemma VLSM_embedding_incl_trans
+  {message}
+  (X : VLSM message)
+  {T : VLSMType message}
+  {MY MZ : VLSMMachine T}
+  (Y := mk_vlsm MY)
+  (Z := mk_vlsm MZ)
+  (project_labelXY : vlabel X -> vlabel Y)
+  (project_stateXY : vstate X -> vstate Y)
+  (ProjXY : VLSM_full_projection X Y project_labelXY project_stateXY)
+  (ProjYZ : VLSM_incl Y Z)
+  : VLSM_full_projection X Z project_labelXY project_stateXY.
+Proof.
+  change project_labelXY with (id ∘ project_labelXY).
+  change project_stateXY with (id ∘ project_stateXY).
+  by apply (VLSM_embedding_trans X Y Z); [| apply VLSM_incl_is_full_projection].
+Qed.
+
+Lemma VLSM_incl_projection_trans
+  {message}
+  {T : VLSMType message}
+  {MX MY : VLSMMachine T}
+  (X := mk_vlsm MX)
+  (Y := mk_vlsm MY)
+  (Z : VLSM message)
+  (ProjXY : VLSM_incl X Y)
+  (project_labelYZ : vlabel Y -> option (vlabel Z))
+  (project_stateYZ : vstate Y -> vstate Z)
+  (ProjYZ : VLSM_projection Y Z project_labelYZ project_stateYZ)
+  : VLSM_projection X Z project_labelYZ project_stateYZ.
+Proof.
+  change project_labelYZ with (project_labelYZ ∘ id).
+  change project_stateYZ with (project_stateYZ ∘ id).
+  apply (VLSM_embedding_projection_trans X Y Z); [| done].
+  by apply VLSM_incl_is_full_projection in ProjXY.
+Qed.
+
+Lemma VLSM_incl_embedding_trans
+  {message}
+  {T : VLSMType message}
+  {MX MY : VLSMMachine T}
+  (X := mk_vlsm MX)
+  (Y := mk_vlsm MY)
+  (Z : VLSM message)
+  (ProjXY : VLSM_incl X Y)
+  (project_labelYZ : vlabel Y -> vlabel Z)
+  (project_stateYZ : vstate Y -> vstate Z)
+  (ProjYZ : VLSM_full_projection Y Z project_labelYZ project_stateYZ)
+  : VLSM_full_projection X Z project_labelYZ project_stateYZ.
+Proof.
+  change project_labelYZ with (project_labelYZ ∘ id).
+  change project_stateYZ with (project_stateYZ ∘ id).
+  apply (VLSM_embedding_trans X Y Z); [| done].
+  by apply VLSM_incl_is_full_projection in ProjXY.
+Qed.
+
+Lemma VLSM_projection_eq_trans
+  {message}
+  (X : VLSM message)
+  {T : VLSMType message}
+  {MY MZ : VLSMMachine T}
+  (Y := mk_vlsm MY)
+  (Z := mk_vlsm MZ)
+  (project_labelXY : vlabel X -> option (vlabel Y))
+  (project_stateXY : vstate X -> vstate Y)
+  (ProjXY : VLSM_projection X Y project_labelXY project_stateXY)
+  (ProjYZ : VLSM_eq Y Z)
+  : VLSM_projection X Z project_labelXY project_stateXY.
+Proof. by apply VLSM_projection_incl_trans; [| apply VLSM_eq_proj1]. Qed.
+
+Lemma VLSM_embedding_eq_trans
+  {message}
+  (X : VLSM message)
+  {T : VLSMType message}
+  {MY MZ : VLSMMachine T}
+  (Y := mk_vlsm MY)
+  (Z := mk_vlsm MZ)
+  (project_labelXY : vlabel X -> vlabel Y)
+  (project_stateXY : vstate X -> vstate Y)
+  (ProjXY : VLSM_full_projection X Y project_labelXY project_stateXY)
+  (ProjYZ : VLSM_eq Y Z)
+  : VLSM_full_projection X Z project_labelXY project_stateXY.
+Proof. by apply VLSM_embedding_incl_trans; [| apply VLSM_eq_proj1]. Qed.
+
+Lemma VLSM_eq_projection_trans
+  {message}
+  {T : VLSMType message}
+  {MX MY : VLSMMachine T}
+  (X := mk_vlsm MX)
+  (Y := mk_vlsm MY)
+  (Z : VLSM message)
+  (ProjXY : VLSM_eq X Y)
+  (project_labelYZ : vlabel Y -> option (vlabel Z))
+  (project_stateYZ : vstate Y -> vstate Z)
+  (ProjYZ : VLSM_projection Y Z project_labelYZ project_stateYZ)
+  : VLSM_projection X Z project_labelYZ project_stateYZ.
+Proof. by apply VLSM_incl_projection_trans; [apply VLSM_eq_proj1 |]. Qed.
+
+Lemma VLSM_eq_embedding_trans
+  {message}
+  {T : VLSMType message}
+  {MX MY : VLSMMachine T}
+  (X := mk_vlsm MX)
+  (Y := mk_vlsm MY)
+  (Z : VLSM message)
+  (ProjXY : VLSM_eq X Y)
+  (project_labelYZ : vlabel Y -> vlabel Z)
+  (project_stateYZ : vstate Y -> vstate Z)
+  (ProjYZ : VLSM_full_projection Y Z project_labelYZ project_stateYZ)
+  : VLSM_full_projection X Z project_labelYZ project_stateYZ.
+Proof. by apply VLSM_incl_embedding_trans; [apply VLSM_eq_proj1 |]. Qed.
+
+End transitivity_props.
